Phi_System/Phi_Type_Algebra.thy
@@ -4309,7 +4309,8 @@ subsubsection \<open>Object Equivalence\<close>
 context begin
 
 private lemma Object_Equiv_rule:
-  \<open> (Ant \<Longrightarrow> \<p>\<r>\<e>\<m>\<i>\<s>\<e> (\<forall>x. eq x x))
+  \<open> Ant \<longrightarrow> Ant' @action \<A>EIF
+\<Longrightarrow> (\<c>\<o>\<n>\<d>\<i>\<t>\<i>\<o>\<n> Ant' \<Longrightarrow> \<p>\<r>\<e>\<m>\<i>\<s>\<e> (\<forall>x. eq x x))
 \<Longrightarrow> (\<And>x. Ant \<longrightarrow> (\<forall>y. eq x y \<longrightarrow> (x \<Ztypecolon> OPEN T \<t>\<r>\<a>\<n>\<s>\<f>\<o>\<r>\<m>\<s> y \<Ztypecolon> MAKE T)) @action \<phi>TA_ind_target undefined)
               \<comment> \<open>Induct over \<open>x \<Ztypecolon> T\<close>. When \<open>x\<close> is inductively split, the constraint of \<open>eq x y\<close>
                   should also split \<open>y\<close>, so that \<open>y \<Ztypecolon> T\<close> can reduce.
@@ -4508,15 +4509,17 @@ subsubsection \<open>Functional Transformation Functor\<close>
 paragraph \<open>Functor\<close>
 
 private lemma \<phi>TA_FTF_rule:
-  \<open> (Ant \<Longrightarrow> Transformation_Functor F1 F2 T U D R mapper)
-\<Longrightarrow> (Ant \<Longrightarrow> Object_Equiv (F2 U) eq)
-\<Longrightarrow> (Ant \<Longrightarrow> \<p>\<r>\<e>\<m>\<i>\<s>\<e> (\<forall>f P x y. mapper (\<lambda>a b. b = f a \<and> P a) x y \<longrightarrow> eq y (fm f P x) \<and> pm f P x))
+  \<open> Ant \<longrightarrow> Ant' @action \<A>EIF
+\<Longrightarrow> (\<c>\<o>\<n>\<d>\<i>\<t>\<i>\<o>\<n> Ant' \<Longrightarrow> Transformation_Functor F1 F2 T U D R mapper)
+\<Longrightarrow> (\<c>\<o>\<n>\<d>\<i>\<t>\<i>\<o>\<n> Ant' \<Longrightarrow> Object_Equiv (F2 U) eq)
+\<Longrightarrow> (\<c>\<o>\<n>\<d>\<i>\<t>\<i>\<o>\<n> Ant' \<Longrightarrow> \<p>\<r>\<e>\<m>\<i>\<s>\<e> (\<forall>f P x y. mapper (\<lambda>a b. b = f a \<and> P a) x y \<longrightarrow> eq y (fm f P x) \<and> pm f P x))
 \<Longrightarrow> \<r>Success
 \<Longrightarrow> \<o>\<b>\<l>\<i>\<g>\<a>\<t>\<i>\<o>\<n> True
 \<Longrightarrow> Ant @action \<phi>TA_ANT
 \<Longrightarrow> Functional_Transformation_Functor F1 F2 T U D R pm fm\<close>
   unfolding Premise_def fun_eq_iff Action_Tag_def
-  using infer_FTF_from_FT .
+  using infer_FTF_from_FT
+  by blast
 
 private lemma \<phi>TA_FTF_deriver_cong:
   \<open> D \<equiv> D'
@@ -4531,16 +4534,18 @@ private lemma \<phi>TA_FTF_deriver_cong:
 paragraph \<open>Bi-Functor\<close>
 
 private lemma \<phi>TA_biFTF_rule:
-  \<open> (Ant \<Longrightarrow> Transformation_BiFunctor F1 F2 T\<^sub>1 T\<^sub>2 U\<^sub>1 U\<^sub>2 D\<^sub>1 D\<^sub>2 R\<^sub>1 R\<^sub>2 mapper)
-\<Longrightarrow> (Ant \<Longrightarrow> Object_Equiv (F2 U\<^sub>1 U\<^sub>2) eq)
-\<Longrightarrow> (Ant \<Longrightarrow> \<p>\<r>\<e>\<m>\<i>\<s>\<e> (\<forall>f\<^sub>1 f\<^sub>2 P\<^sub>1 P\<^sub>2 x y. mapper (\<lambda>a b. b = f\<^sub>1 a \<and> P\<^sub>1 a) (\<lambda>a b. b = f\<^sub>2 a \<and> P\<^sub>2 a) x y
+  \<open> Ant \<longrightarrow> Ant' @action \<A>EIF
+\<Longrightarrow> (\<c>\<o>\<n>\<d>\<i>\<t>\<i>\<o>\<n> Ant' \<Longrightarrow> Transformation_BiFunctor F1 F2 T\<^sub>1 T\<^sub>2 U\<^sub>1 U\<^sub>2 D\<^sub>1 D\<^sub>2 R\<^sub>1 R\<^sub>2 mapper)
+\<Longrightarrow> (\<c>\<o>\<n>\<d>\<i>\<t>\<i>\<o>\<n> Ant' \<Longrightarrow> Object_Equiv (F2 U\<^sub>1 U\<^sub>2) eq)
+\<Longrightarrow> (\<c>\<o>\<n>\<d>\<i>\<t>\<i>\<o>\<n> Ant' \<Longrightarrow> \<p>\<r>\<e>\<m>\<i>\<s>\<e> (\<forall>f\<^sub>1 f\<^sub>2 P\<^sub>1 P\<^sub>2 x y. mapper (\<lambda>a b. b = f\<^sub>1 a \<and> P\<^sub>1 a) (\<lambda>a b. b = f\<^sub>2 a \<and> P\<^sub>2 a) x y
                                   \<longrightarrow> eq y (fm f\<^sub>1 f\<^sub>2 P\<^sub>1 P\<^sub>2 x) \<and> pm f\<^sub>1 f\<^sub>2 P\<^sub>1 P\<^sub>2 x))
 \<Longrightarrow> \<r>Success
 \<Longrightarrow> \<o>\<b>\<l>\<i>\<g>\<a>\<t>\<i>\<o>\<n> True
 \<Longrightarrow> Ant @action \<phi>TA_ANT
 \<Longrightarrow> Functional_Transformation_BiFunctor F1 F2 T\<^sub>1 T\<^sub>2 U\<^sub>1 U\<^sub>2 D\<^sub>1 D\<^sub>2 R\<^sub>1 R\<^sub>2 pm fm\<close>
   unfolding Premise_def fun_eq_iff Action_Tag_def
-  using infer_biFTF_from_biFT .
+  using infer_biFTF_from_biFT
+  by blast
 
 private lemma \<phi>TA_biFTF_deriver_cong:
   \<open> D\<^sub>1 \<equiv> D'\<^sub>1
