Phi_System/Phi_Types.thy
@@ -120,7 +120,7 @@ ML \<open>assert_derived_properties \<^theory> [
 subsection \<open>Func\<close>
 
 declare [[\<phi>trace_reasoning = 0]]
-  
+
 \<phi>type_def \<phi>Fun :: \<open>('a \<Rightarrow> 'c) \<Rightarrow> ('c,'a) \<phi>\<close>
   where \<open>\<phi>Fun f x = (f x \<Ztypecolon> Itself)\<close>
   opening  extract_premises_in_local_inverse
@@ -129,6 +129,7 @@ declare [[\<phi>trace_reasoning = 0]]
        and Basic
        and Functionality
        and Abstraction_to_Raw
+
 
 (*The assertions are used to test the property derivers. As the deriviers are changed frequently
   during the development, the assertions check and report if any mistakes are introduced by comparing
@@ -1480,7 +1481,7 @@ ML \<open>assert_derived_properties \<^theory> [
   (@{thm' \<phi>Fun'.Object_Equiv}, \<^pattern_prop>\<open> Object_Equiv ?T ?eq \<Longrightarrow> Object_Equiv (?f \<Zcomp>\<^sub>f ?T) ?eq \<close>),
   (@{thm' \<phi>Fun'.Transformation_Functor}, \<^pattern_prop>\<open>\<g>\<u>\<a>\<r>\<d> \<c>\<o>\<n>\<d>\<i>\<t>\<i>\<o>\<n> ?f = ?fa \<Longrightarrow> Transformation_Functor ((\<Zcomp>\<^sub>f) ?f) ((\<Zcomp>\<^sub>f) ?fa) ?T ?U (\<lambda>a. {a}) (\<lambda>_. UNIV) (\<lambda>a. a)  \<close>),
   (@{thm' \<phi>Fun'.Functional_Transformation_Functor}, \<^pattern_prop>\<open>\<g>\<u>\<a>\<r>\<d> \<c>\<o>\<n>\<d>\<i>\<t>\<i>\<o>\<n> ?f = ?fa \<Longrightarrow> Functional_Transformation_Functor ((\<Zcomp>\<^sub>f) ?f) ((\<Zcomp>\<^sub>f) ?fa) ?T ?U (\<lambda>a. {a}) (\<lambda>_. UNIV) (\<lambda>f a. a) (\<lambda>f P. f) \<close>),
-  (@{thm' \<phi>Fun'.\<phi>Sum_Comm\<^sub>E}, \<^pattern_prop>\<open>\<g>\<u>\<a>\<r>\<d> \<c>\<o>\<n>\<d>\<i>\<t>\<i>\<o>\<n> ?f = ?fa \<and> ?fa = ?faa \<Longrightarrow>
+  (@{thm' \<phi>Fun'.\<phi>Sum_Comm\<^sub>E}, \<^pattern_prop>\<open>\<g>\<u>\<a>\<r>\<d> \<c>\<o>\<n>\<d>\<i>\<t>\<i>\<o>\<n> ?f = ?fa \<and> ?f = ?faa \<Longrightarrow>
         Tyops_Commute\<^sub>1\<^sub>_\<^sub>2 ((\<Zcomp>\<^sub>f) ?f) ((\<Zcomp>\<^sub>f) ?fa) ((\<Zcomp>\<^sub>f) ?faa) (+\<^sub>\<phi>) (+\<^sub>\<phi>) ?T ?U (\<lambda>x. True) (embedded_func (\<lambda>x. x) (\<lambda>x. True))  \<close>),
   (@{thm' \<phi>Fun'.Open_Abstraction_to_Raw}, \<^pattern_prop>\<open> (\<And>x. x \<Ztypecolon> ?T \<t>\<r>\<a>\<n>\<s>\<f>\<o>\<r>\<m>\<s> y \<Ztypecolon> (Itself::(?'c2,?'c2) \<phi>) \<s>\<u>\<b>\<j> y. ?r x y @action to (Itself::(?'c2,?'c2) \<phi>))
                                                     \<Longrightarrow> ?x \<Ztypecolon> ?f \<Zcomp>\<^sub>f ?T \<t>\<r>\<a>\<n>\<s>\<f>\<o>\<r>\<m>\<s> y \<Ztypecolon> (Itself::(?'c,?'c) \<phi>) \<s>\<u>\<b>\<j> y. (\<exists>x. y = ?f x \<and> ?r ?x x) @action to (Itself::(?'c,?'c) \<phi>)  \<close>),
@@ -1799,7 +1800,7 @@ ML \<open>assert_derived_properties \<^theory> [
   (@{thm' \<phi>ScalarMul.\<phi>Fun'_Comm\<^sub>I}, \<^pattern_prop>\<open> fun_commute (scalar_mult ?f ?s) ?fa (scalar_mult ?xa ?xb) ?xc \<Longrightarrow>
     Tyops_Commute (\<phi>ScalarMul ?f ?s) (\<phi>ScalarMul ?xa ?xb) ((\<Zcomp>\<^sub>f) ?fa) ((\<Zcomp>\<^sub>f) ?xc) ?Ta (\<lambda>x. True) (embedded_func (\<lambda>x. x) (\<lambda>_. True))  \<close>),
   (@{thm' \<phi>ScalarMul.\<phi>Sum_Comm\<^sub>E}, \<^pattern_prop>\<open>
-      \<g>\<u>\<a>\<r>\<d> \<c>\<o>\<n>\<d>\<i>\<t>\<i>\<o>\<n> (?s = ?sa \<and> ?f = ?fa) \<and> ?sa = ?saa \<and> ?fa = ?faa \<Longrightarrow>
+      \<g>\<u>\<a>\<r>\<d> \<c>\<o>\<n>\<d>\<i>\<t>\<i>\<o>\<n> (?s = ?sa \<and> ?f = ?fa) \<and> ?s = ?saa \<and> ?f = ?faa \<Longrightarrow>
       Tyops_Commute\<^sub>1\<^sub>_\<^sub>2 (\<phi>ScalarMul ?f ?s) (\<phi>ScalarMul ?fa ?sa) (\<phi>ScalarMul ?faa ?saa) (+\<^sub>\<phi>) (+\<^sub>\<phi>) ?T ?U (\<lambda>x. True)
        (embedded_func (\<lambda>x. x) (\<lambda>x. True)) \<close>),
   (@{thm' \<phi>ScalarMul.Make_Abstraction_from_Raw}, \<^pattern_prop>\<open> ?c \<Ztypecolon> Itself \<t>\<r>\<a>\<n>\<s>\<f>\<o>\<r>\<m>\<s> ?y \<Ztypecolon> ?T \<Longrightarrow> scalar_mult ?f ?s ?c \<Ztypecolon> Itself \<t>\<r>\<a>\<n>\<s>\<f>\<o>\<r>\<m>\<s> ?y \<Ztypecolon> \<s>\<c>\<a>\<l>\<a>\<r>[?f] ?s \<Zcomp> ?T \<close>),
